starting graph module

examples.dfy
@@ -81,17 +81,3 @@ module Distributive {
         assert count([true, true]) == 2;
     }
 }
-
-module Graphs {
-    class Node {
-        var next: seq<Node>;
-    }
-
-    predicate closed(graph: set<Node>) 
-    reads graph
-    {
-        forall i :: i in graph ==> 
-            forall k :: 0 <= k < |i.next| ==> i.next[k] in graph 
-                                                && i.next[k] != i
-    }
-}
